Eliminate admits in globals using new hex encoding

new/golang/theory/globals.v
@@ -1,7 +1,7 @@
 From New.golang.theory Require Import exception mem typing.
 From New.golang.defn Require Import globals.
 From iris.base_logic.lib Require Import ghost_map ghost_var.
-From Coq Require Import Ascii.
+From Coq Require Import Ascii Equality.
 
 Class goGlobals_preG `{ffi_syntax} (Σ: gFunctors) : Set :=
   {
@@ -19,7 +19,8 @@ Class goGlobalsGS `{ffi_syntax} Σ : Set :=
     }.
 
 Definition goGlobalsΣ `{ffi_syntax} : gFunctors :=
-  #[ghost_mapΣ (go_string * go_string) loc ; ghost_mapΣ go_string (); ghost_varΣ (option (gmap go_string val))].
+  #[ghost_mapΣ (go_string * go_string) loc ; ghost_mapΣ go_string ();
+    ghost_varΣ (option (gmap go_string val))].
 
 Global Instance subG_goGlobalsG `{ffi_syntax} {Σ} : subG goGlobalsΣ Σ → goGlobals_preG Σ.
 Proof. solve_inG. Qed.
@@ -28,25 +29,14 @@ Section definitions_and_lemmas.
 Context `{ffi_sem: ffi_semantics} `{!ffi_interp ffi} `{!heapGS Σ}.
 Context `{!goGlobalsGS Σ}.
 
-Fixpoint is_valid_package_name (pkg_name : go_string) : bool :=
-  match pkg_name with
-  | [] => true
-  | {| Naive.unsigned := 32; Naive._unsigned_in_range := eq_refl |} :: _ => false
-    (* Check " "%go. *)
-  | _ :: pkg_name => is_valid_package_name pkg_name
-  end.
-
-Local Notation encode_var_name := (globals.globals.encode_var_name).
-
 (* The only concurrent access to globals is to read the address of global
    variables, so that's the only thing this invariant is concerned with. *)
 Local Definition own_globals_inv : iProp Σ :=
   ∃ g (addrs : gmap (go_string * go_string) loc),
   "Hglobals_i" ∷ own_globals (DfracOwn (1/2)) g ∗
   "Haddrs" ∷ ghost_map_auth go_globals_name 1%Qp addrs ∗
-  "%Hvars" ∷ (⌜ ∀ pkg_name var_name,
-                is_valid_package_name pkg_name →
-                # <$> addrs !! (pkg_name, var_name) = g !! (encode_var_name pkg_name var_name) ⌝).
+  "%Hvars" ∷ (⌜ # <$> kmap globals.encode_var addrs ⊆ g ⌝)
+.
 
 Local Definition is_globals_inv : iProp Σ :=
   inv nroot own_globals_inv.
@@ -58,12 +48,11 @@ Definition own_globals_tok_def (pending_packages : gset go_string)
   "Hglobals" ∷ own_globals (DfracOwn (1/2)) g ∗
   "Hacc" ∷ ghost_var go_access_prev_state_name 1%Qp None ∗
   "%Hpkg" ∷ (⌜ ∀ pkg_name,
-               is_valid_package_name pkg_name →
                pkg_name ∈ pending_packages ∨
                  (match pkg_initialized !! pkg_name with
-                  | Some _ => g !! pkg_name = Some #()%V
-                  | None => g !! pkg_name = None ∧
-                           ∀ var_name, g !! (encode_var_name pkg_name var_name) = None
+                  | Some _ => g !! globals.encode_package pkg_name = Some #()%V
+                  | None => g !! globals.encode_package pkg_name = None ∧
+                           ∀ var_name, g !! (globals.encode_var (pkg_name, var_name)) = None
                   end) ⌝) ∗
   "#Hinv" ∷ is_globals_inv ∗
   "#Hinited" ∷ ([∗ map] pkg_name ↦ _ ∈ pkg_initialized,
@@ -90,19 +79,20 @@ Definition is_initialized_def (pkg_name : go_string) (P : iProp Σ) : iProp Σ :
 Program Definition is_initialized := unseal (_:seal (@is_initialized_def)). Obligation 1. by eexists. Qed.
 Definition is_initialized_unseal : is_initialized = _ := seal_eq _.
 
-Definition is_global_addr_def (var_id : go_string * go_string) (addr : loc) : iProp Σ :=
-  is_globals_inv ∗ var_id ↪[go_globals_name]□ addr ∗ ⌜ is_valid_package_name var_id.1 ⌝.
+Definition is_global_addr_def (pkg_var_name : go_string * go_string) (addr : loc) : iProp Σ :=
+  is_globals_inv ∗ pkg_var_name ↪[go_globals_name]□ addr.
 Program Definition is_global_addr := unseal (_:seal (@is_global_addr_def)). Obligation 1. by eexists. Qed.
 Definition is_global_addr_unseal : is_global_addr = _ := seal_eq _.
 
-Definition own_unused_vars_def (pkg_name : go_string) (used_var_names : gset go_string) : iProp Σ :=
+Definition own_unused_vars_def (pkg_name : go_string) (used_pkg_vars : gset (go_string * go_string)) :
+  iProp Σ :=
   ∃ g_old var_addrs,
-  "Hglobals" ∷ own_globals (DfracOwn (1/2)) ((kmap (encode_var_name pkg_name) var_addrs) ∪ g_old) ∗
+  "Hglobals" ∷ own_globals (DfracOwn (1/2)) ((kmap globals.encode_var var_addrs) ∪ g_old) ∗
   "Hacc" ∷ ghost_var go_access_prev_state_name (1/2)%Qp (Some g_old) ∗
   "#Hinv" ∷ is_globals_inv ∗
-  "%Hused_vars_dom" ∷ (⌜ dom var_addrs = used_var_names ⌝) ∗
-  "%Hvalid" ∷ ⌜ is_valid_package_name pkg_name ⌝ ∗
-  "%Hold_unused" ∷ (⌜ ∀ var_name, g_old !! (encode_var_name pkg_name var_name) = None ⌝).
+  "%Hused_vars_dom" ∷ (⌜ dom var_addrs = used_pkg_vars ⌝) ∗
+  "%Hused_pkg" ∷ (⌜ ∀ pkg_var_name, pkg_var_name ∈ used_pkg_vars → pkg_var_name.1 = pkg_name ⌝) ∗
+  "%Hold_unused" ∷ (⌜ ∀ var_name, g_old !! (globals.encode_var (pkg_name, var_name)) = None ⌝).
 Program Definition own_unused_vars := unseal (_:seal (@own_unused_vars_def)). Obligation 1. by eexists. Qed.
 Definition own_unused_vars_unseal : own_unused_vars = _ := seal_eq _.
 
@@ -150,27 +140,142 @@ Proof.
   by iMod ("Hclose" with "[$Htok]").
 Qed.
 
-Lemma encode_var_name_inj pkg_name1 pkg_name2 var_name1 var_name2 :
-  is_valid_package_name pkg_name1 →
-  is_valid_package_name pkg_name2 →
-  encode_var_name pkg_name1 var_name1 = encode_var_name pkg_name2 var_name2 →
-  pkg_name1 = pkg_name2 ∧ var_name1 = var_name2.
+Lemma hex_encode_length (w : w8) :
+  length (globals.hex_encode_w8 w) = 2%nat.
 Proof.
-Admitted.
+  rewrite -(ByteString.w8_to_byte_to_w8 w).
+  generalize (w8_to_byte w). clear.
+  by intros [].
+Qed.
 
-Lemma encode_var_name_package_name_ne pkg_name' pkg_name var_name :
-  is_valid_package_name pkg_name' →
-  pkg_name' ≠ encode_var_name pkg_name var_name.
+Local Definition hex := ["00";"01";"02";"03";"04";"05";"06";"07";"08";"09";"0a";"0b";"0c";"0d";"0e";"0f";"10";"11";"12";"13";"14";"15";"16";"17";"18";"19";"1a";"1b";"1c";"1d";"1e";"1f";"20";"21";"22";"23";"24";"25";"26";"27";"28";"29";"2a";"2b";"2c";"2d";"2e";"2f";"30";"31";"32";"33";"34";"35";"36";"37";"38";"39";"3a";"3b";"3c";"3d";"3e";"3f";"40";"41";"42";"43";"44";"45";"46";"47";"48";"49";"4a";"4b";"4c";"4d";"4e";"4f";"50";"51";"52";"53";"54";"55";"56";"57";"58";"59";"5a";"5b";"5c";"5d";"5e";"5f";"60";"61";"62";"63";"64";"65";"66";"67";"68";"69";"6a";"6b";"6c";"6d";"6e";"6f";"70";"71";"72";"73";"74";"75";"76";"77";"78";"79";"7a";"7b";"7c";"7d";"7e";"7f";"80";"81";"82";"83";"84";"85";"86";"87";"88";"89";"8a";"8b";"8c";"8d";"8e";"8f";"90";"91";"92";"93";"94";"95";"96";"97";"98";"99";"9a";"9b";"9c";"9d";"9e";"9f";"a0";"a1";"a2";"a3";"a4";"a5";"a6";"a7";"a8";"a9";"aa";"ab";"ac";"ad";"ae";"af";"b0";"b1";"b2";"b3";"b4";"b5";"b6";"b7";"b8";"b9";"ba";"bb";"bc";"bd";"be";"bf";"c0";"c1";"c2";"c3";"c4";"c5";"c6";"c7";"c8";"c9";"ca";"cb";"cc";"cd";"ce";"cf";"d0";"d1";"d2";"d3";"d4";"d5";"d6";"d7";"d8";"d9";"da";"db";"dc";"dd";"de";"df";"e0";"e1";"e2";"e3";"e4";"e5";"e6";"e7";"e8";"e9";"ea";"eb";"ec";"ed";"ee";"ef";"f0";"f1";"f2";"f3";"f4";"f5";"f6";"f7";"f8";"f9";"fa";"fb";"fc";"fd";"fe";"ff"]%go.
+Local Lemma hex_NoDup_helper : hex = remove_dups hex.
+Proof. reflexivity. Qed.
+Local Lemma hex_NoDup : NoDup hex.
+Proof. rewrite hex_NoDup_helper. apply NoDup_remove_dups. Qed.
+Local Definition hex_encode_w8' (x : w8) := default "00"%go (hex !! uint.nat x).
+Local Lemma hex_encode_eq (x : w8) : hex_encode_w8' x = globals.hex_encode_w8 x.
 Proof.
-Admitted.
+  rewrite -(ByteString.w8_to_byte_to_w8 x).
+  generalize (w8_to_byte x) as x'. clear. by intros [].
+Qed.
+Local Lemma hex_lookup (x : w8) :
+  ∃ y, hex !! (uint.nat x) = Some y.
+Proof.
+  destruct (hex !! _) eqn:Hbad.
+  { by eexists. }
+  exfalso.
+  rewrite lookup_ge_None /= in Hbad.
+  word.
+Qed.
 
-Lemma wp_globals_put var_id used_var_names (addr : loc) :
-  var_id.2 ∉ used_var_names →
-  {{{ own_unused_vars var_id.1 used_var_names }}}
-    globals.put var_id #addr
+Delimit Scope byte_char_scope with go_byte.
+
+Local Definition hex_chars :=
+  ["0"; "1"; "2"; "3"; "4"; "5"; "6"; "7"; "8"; "9"; "a"; "b"; "c"; "d"; "e"; "f" ]%go_byte.
+
+Lemma hex_encode_subseteq x : (globals.hex_encode x ⊆ hex_chars).
+Proof.
+  induction x.
+  { set_solver. }
+  simpl.
+  rewrite -hex_encode_eq.
+  rewrite list_subseteq_app_iff_l.
+  split; try done.
+  rewrite -(ByteString.w8_to_byte_to_w8 a).
+  generalize (w8_to_byte a) as x'. clear.
+  intros [].
+  1-50: set_solver.
+  1-50: set_solver.
+  1-50: set_solver.
+  1-50: set_solver.
+  1-50: set_solver.
+  all: set_solver.
+Qed.
+
+Instance hex_encode_w8_inj : Inj (=) (=) globals.hex_encode_w8.
+Proof.
+  hnf. intros x y.
+  rewrite -!hex_encode_eq.
+  intros Heq.
+  rewrite /hex_encode_w8' in Heq.
+  pose proof (hex_lookup x) as [? Hl1].
+  pose proof (hex_lookup y) as [? Hl2].
+  rewrite Hl1 Hl2 /= in Heq. subst.
+  apply word.unsigned_inj.
+  apply Z2Nat.inj; try word.
+  eapply NoDup_lookup; try done.
+  apply hex_NoDup.
+Qed.
+
+Lemma hex_encode_w8_length x : length (globals.hex_encode_w8 x) = 2.
+Proof.
+  rewrite -(ByteString.w8_to_byte_to_w8 x).
+  generalize (w8_to_byte x) as x'. clear. by intros [].
+Qed.
+
+Instance hex_encode_inj : Inj (=) (=) globals.hex_encode.
+Proof.
+  hnf. intros.
+  move x after y.
+  dependent induction x generalizing y.
+  { destruct y; first done.
+    exfalso. apply (f_equal length) in H.
+    rewrite /= length_app hex_encode_length in H. lia.
+  }
+  destruct y.
+  { exfalso. apply (f_equal length) in H.
+    rewrite /= length_app hex_encode_length in H. lia. }
+  simpl in H.
+  apply app_inj_1 in H.
+  2:{ rewrite !hex_encode_w8_length //. }
+  intuition.
+  f_equal.
+  - by apply hex_encode_w8_inj.
+  - by apply IHx.
+Qed.
+
+Lemma encode_package_inj pkg_name1 pkg_name2 :
+  globals.encode_package pkg_name1 = globals.encode_package pkg_name2 →
+  pkg_name1 = pkg_name2.
+Proof.
+  intros Heq.
+  apply app_inv_head in Heq.
+  by apply hex_encode_inj.
+Qed.
+
+Local Instance encode_var_inj : Inj (=) (=) globals.encode_var.
+Proof.
+  intros pkg_name pkg_name' Heq.
+  apply app_inv_head in Heq.
+  change (" "%go) with ([" "%go_byte]) in Heq.
+  rewrite -!cons_middle in Heq.
+  apply app_inj_pivot in Heq as [Hbad|Heq].
+  {
+    exfalso.
+    rewrite -!elem_of_list_In in Hbad.
+    pose proof (hex_encode_subseteq pkg_name.1).
+    pose proof (hex_encode_subseteq pkg_name.2).
+    set_solver.
+  }
+  intuition.
+  repeat match goal with
+  | [ H : context [globals.hex_encode] |- _] => apply (hex_encode_inj) in H
+  end. destruct pkg_name, pkg_name'.
+  simpl in *. subst. done.
+Qed.
+
+Lemma encode_var_name_package_name_ne pkg_name pkg_var_name :
+  globals.encode_package pkg_name ≠ globals.encode_var pkg_var_name.
+Proof. done. Qed.
+
+Lemma wp_globals_put pkg_var_name used_pkg_vars (addr : loc) :
+  pkg_var_name ∉ used_pkg_vars →
+  {{{ own_unused_vars pkg_var_name.1 used_pkg_vars }}}
+    globals.put pkg_var_name #addr
   {{{ RET #();
-      own_unused_vars var_id.1 ({[ var_id.2 ]} ∪ used_var_names) ∗
-      is_global_addr var_id addr
+      own_unused_vars pkg_var_name.1 ({[ pkg_var_name ]} ∪ used_pkg_vars) ∗
+      is_global_addr pkg_var_name addr
   }}}.
 Proof.
   iIntros (??) "Hu HΦ".
@@ -183,41 +288,28 @@ Proof.
   iInv "Hinv" as "Hi" "Hclose".
   iMod (lc_fupd_elim_later with "Hlc Hi") as "Hi".
   iNamed "Hi".
-  iCombine "Hglobals Hglobals_i" gives %[_ <-].
+  iCombine "Hglobals Hglobals_i" gives %[_ Heq]. subst.
   iCombine "Hglobals Hglobals_i" as "Hglobals".
   iApply (wp_GlobalPut with "[$]").
   iNext. iIntros "Hglobals".
-  iMod (ghost_map_insert_persist var_id with "Haddrs") as "[Haddrs #Hptsto]".
+  iMod (ghost_map_insert_persist pkg_var_name addr with "Haddrs")
+    as "[Haddrs #Hptsto]".
   {
-    subst.
-    specialize (Hvars var_id.1 var_id.2 ltac:(assumption)).
-    rewrite lookup_union lookup_kmap (not_elem_of_dom_1 var_addrs)
-      //= left_id Hold_unused fmap_None in Hvars.
-    by destruct var_id.
+    eapply lookup_weaken_None in Hvars.
+    { rewrite lookup_fmap fmap_None // in Hvars.
+      erewrite lookup_kmap in Hvars.
+      - done.
+      - apply _.
+    }
+    rewrite lookup_union lookup_kmap Hold_unused.
+    rewrite (not_elem_of_dom_1 var_addrs) //.
   }
   iDestruct "Hglobals" as "[Hglobals Hglobals_i]".
   iMod ("Hclose" with "[-HΦ Hglobals Hacc]") as "_".
   {
     iFrame "∗#%". iPureIntro.
-    intros.
-    destruct (decide ((pkg_name, var_name) = var_id)).
-    {
-      subst.
-      rewrite !lookup_insert /=.
-      rewrite to_val_unseal //.
-    }
-    {
-      rewrite lookup_insert_ne //.
-      rewrite lookup_insert_ne //.
-      2:{
-        intros Hbad.
-        apply n.
-        apply encode_var_name_inj in Hbad; try done.
-        intuition; subst.
-        by destruct var_id.
-      }
-      by apply Hvars.
-    }
+    rewrite kmap_insert fmap_insert [in #addr]to_val_unseal /=.
+    by apply insert_mono.
   }
   iApply "HΦ".
   rewrite insert_union_l -kmap_insert.
@@ -226,15 +318,14 @@ Proof.
   set_solver.
 Qed.
 
-Lemma wp_globals_get var_id (addr : loc) :
-  {{{ is_global_addr var_id addr }}}
-    globals.get var_id #()
+Lemma wp_globals_get pkg_var_name (addr : loc) :
+  {{{ is_global_addr pkg_var_name addr }}}
+    globals.get pkg_var_name #()
   {{{ RET #addr; True }}}.
 Proof.
   unseal.
   iIntros (?) "Hu HΦ".
-  destruct var_id as [pkg_name var_name].
-  iDestruct "Hu" as "(#Hinv & #Haddr & %Hvalid)".
+  iDestruct "Hu" as "(#Hinv & #Haddr)".
   wp_call_lc "Hlc".
   wp_bind (GlobalGet _).
   iInv "Hinv" as "Hi" "Hclose".
@@ -244,14 +335,14 @@ Proof.
   iApply (wp_GlobalGet with "[$]").
   iNext. iIntros.
   iCombine "Haddrs Haddr" gives %Hlookup.
-  rewrite -Hvars // Hlookup.
+  erewrite lookup_weaken; try eassumption.
+  2:{ rewrite lookup_fmap lookup_kmap Hlookup //. }
   iMod ("Hclose" with "[-HΦ]").
   { iFrame "∗#%". }
   iModIntro. wp_pures. by iApply "HΦ".
 Qed.
 
 Lemma wp_package_init pending postconds (pkg_name : go_string) (init_func : val) P Φ :
-  is_valid_package_name pkg_name →
   postconds !! pkg_name = Some P →
   pkg_name ∉ pending →
   own_globals_tok pending postconds -∗
@@ -266,7 +357,7 @@ Lemma wp_package_init pending postconds (pkg_name : go_string) (init_func : val)
   WP (globals.package_init pkg_name init_func) {{ Φ }}.
 Proof.
   unseal.
-  intros Hvalid Hpost Hnot_pending.
+  intros Hpost Hnot_pending.
   iIntros "Htok Hinit HΦ".
   wp_call.
   iNamed "Htok".
@@ -274,10 +365,10 @@ Proof.
   rewrite [in GlobalGet _]to_val_unseal.
   iApply (wp_GlobalGet with "[$]").
   iNext. iIntros "Hglobals".
-  destruct (lookup pkg_name g) eqn:Hlookup; rewrite Hlookup.
+  destruct (lookup (globals.encode_package pkg_name) g) eqn:Hlookup; rewrite Hlookup.
   { (* don't bother running init *)
     wp_pures.
-    pose proof (Hpkg pkg_name ltac:(done)) as Hpkg'.
+    pose proof (Hpkg pkg_name) as Hpkg'.
     rewrite Hlookup /= in Hpkg'.
     destruct Hpkg' as [|Hpkg']; first done.
     destruct (pkg_initialized !! pkg_name) as [[]|] eqn:Hpkg_lookup; last naive_solver.
@@ -302,7 +393,7 @@ Proof.
     iFrame.
     iPureIntro.
     split; first done.
-    specialize (Hpkg pkg_name ltac:(done)).
+    specialize (Hpkg pkg_name).
     destruct Hpkg as [|Hpkg]; first done.
     destruct (pkg_initialized !! pkg_name); first naive_solver.
     destruct Hpkg as [_ Hnone].
@@ -312,20 +403,20 @@ Proof.
   {
     iRename "Hacc" into "Hacc2".
     rename g into g_old.
-    clear Hvalid. iClear "Hinv".
+    iClear "Hinv".
     iIntros (?). iNamed 1.
-    iCombine "Hacc Hacc2" gives %[_ Heq].
-    inversion_clear Heq.
+    iCombine "Hacc Hacc2" gives %[_ [=Heq]].
+    subst.
     iCombine "Hacc Hacc2" as "Hacc".
     iMod (ghost_var_update None with "Hacc") as "Hacc".
     iModIntro.
     iFrame "∗#%".
     iPureIntro.
-    intros pkg_name' Hvalid'.
+    intros pkg_name'.
     destruct (decide (pkg_name' ∈ {[pkg_name]} ∪ pending)).
     { by left. }
     right.
-    specialize (Hpkg pkg_name' ltac:(done)).
+    specialize (Hpkg pkg_name').
     destruct Hpkg as [|Hpkg].
     { set_solver. }
     destruct (pkg_initialized !! pkg_name').
@@ -343,9 +434,11 @@ Proof.
       {
         intros.
         rewrite lookup_union_r //.
-        rewrite lookup_kmap_None.
-        intros. exfalso. apply encode_var_name_inj in H0; try done.
-        set_solver.
+        rewrite lookup_kmap.
+        rewrite -not_elem_of_dom.
+        intros Hin.
+        specialize (Hused_pkg (pkg_name', var_name) ltac:(done)).
+        subst. set_solver.
       }
     }
   }
@@ -366,9 +459,9 @@ Proof.
   iMod ("Hclose" with "[Hglobals_i Haddrs]").
   {
     iFrame "∗#%". iPureIntro.
-    setoid_rewrite lookup_insert_ne.
-    { done. }
-    by apply encode_var_name_package_name_ne.
+    apply insert_subseteq_r; try done.
+    rewrite lookup_fmap fmap_None lookup_kmap_None.
+    intros. exfalso. by eapply encode_var_name_package_name_ne.
   }
   iMod (inv_alloc with "[HP]") as "#Hinit";
     last iSpecialize ("HΦ" with "Hinit").
@@ -378,8 +471,8 @@ Proof.
   { simpl. rewrite Hpost. iFrame "#". }
   iFrame "∗#%".
   iPureIntro.
-  intros pkg_name' ?.
-  specialize (Hpkg pkg_name' ltac:(done)).
+  intros pkg_name'.
+  specialize (Hpkg pkg_name').
   destruct (decide (pkg_name' = pkg_name)).
   {
     subst. right.
@@ -390,8 +483,9 @@ Proof.
   right.
   rewrite lookup_insert_ne //.
   destruct (_ !! pkg_name').
-  { rewrite lookup_insert_ne //. }
+  { rewrite lookup_insert_ne //. intros H. eapply encode_package_inj in H. done. }
   rewrite lookup_insert_ne //.
+  2:{ intros H. eapply encode_package_inj in H. done. }
   destruct Hpkg as [? ?].
   split; first done.
   setoid_rewrite lookup_insert_ne.
@@ -431,7 +525,7 @@ Proof.
   iNext.
   iFrame.
   iPureIntro. intros.
-  rewrite !lookup_empty //.
+  rewrite kmap_empty fmap_empty //.
 Qed.
 
 End init.
